src/3d/Options.fst
@@ -115,6 +115,8 @@ let emit_output_types_defs : ref bool = alloc true
 
 let emit_smt_encoding : ref bool = alloc false
 
+let z3_diff_test: ref (option (valid_string valid_equate_types)) = alloc None
+
 let z3_test : ref (option vstring) = alloc None
 
 let z3_witnesses : ref (option vstring) = alloc None
@@ -351,6 +353,7 @@ let (display_usage_2, compute_options_2, fstar_options) =
     CmdOption "skip_o_rules" (OptBool skip_o_rules) "With --makefile, do not generate rules for .o files" [];
     CmdFStarOption (let open FStar.Getopt in noshort, "version", ZeroArgs (fun _ -> FStar.IO.print_string (Printf.sprintf "EverParse/3d %s\nCopyright 2018, 2019, 2020 Microsoft Corporation\n" Version.everparse_version); exit 0), "Show this version of EverParse");
     CmdOption "equate_types" (OptList "an argument of the form A,B, to generate asserts of the form (A.t == B.t)" valid_equate_types equate_types_list) "Takes an argument of the form A,B and then for each entrypoint definition in B, it generates an assert (A.t == B.t) in the B.Types file, useful when refactoring specs, you can provide multiple equate_types on the command line" [];
+    CmdOption "z3_diff_test" (OptStringOption "parser1,parser2" valid_equate_types z3_diff_test) "produce differential tests for two parsers" [];
     CmdOption "z3_test" (OptStringOption "parser name" always_valid z3_test) "produce positive and negative test cases for a given parser" [];
     CmdOption "z3_witnesses" (OptStringOption "nb" always_valid z3_witnesses) "ask for nb distinct test witnesses" [];
     CmdOption "__arg0" (OptStringOption "executable name" always_valid arg0) "executable name to use for the help message" [];
@@ -530,3 +533,8 @@ let get_z3_witnesses () =
   with _ -> 1
 
 let get_debug _ = !debug
+
+let get_z3_diff_test _ =
+  match !z3_diff_test with
+  | None -> None
+  | Some s -> let [p1; p2] = String.split [','] s in Some (p1, p2)
