src/3d/Options.fsti
@@ -69,3 +69,5 @@ val get_z3_test: unit -> ML (option string)
 val get_z3_witnesses: unit -> ML int
 
 val get_debug: unit -> ML bool
+
+val get_z3_diff_test: unit -> ML (option (string & string))
